backends/lean/Aeneas/Std/Spec.lean
@@ -1,0 +1,74 @@
+import Lean
+import AeneasMeta.Extensions
+-- import Aeneas.Tactic.Step.Init
+open Lean Elab Term Meta
+
+namespace Aeneas
+open Extensions
+
+-- This file defines an extension for defining spec statements that
+-- can be used with the step tactic.
+
+-- structure SpecInfo where
+--   name : Lean.Name
+--   arity : Nat
+--   mk_spec_mono : Array Lean.Expr → Lean.Expr → Lean.Expr
+--   mk_spec_bind : Array Lean.Expr → Lean.Expr → Lean.Expr
+--   -- discr_tree_key : Array Lean.Expr → Array Lean.Expr
+--   program_index : Nat -- index into the arguments of the Result value
+
+--   uncurry_elim_tactics : Array Lean.Name
+--   qimp_elim_tactics : Array Lean.Name
+--   deriving Inhabited -- why does the value type for an extension need to be Inhabited?
+
+-- structure SpecInfoExtensionState where
+--   specInfos : Std.HashMap Name SpecInfo
+
+-- /- Initiliaze the `spec` attribute. -/
+-- initialize specAttr : SimpleScopedEnvExtension SpecInfo SpecInfoExtensionState ← do
+--   let ext ← registerSimpleScopedEnvExtension {
+--     name        := `specStatementRegistrationExtension,
+--     initial     := {
+--       specInfos := Std.HashMap.emptyWithCapacity
+--     },
+--     addEntry    := fun state new =>
+--       {state with specInfos := state.specInfos.insert new.name new},
+--   }
+--   pure ext
+
+-- syntax (name := register_spec_statement_cmd)
+--   "#register_spec_statement " term : command
+
+-- @[command_elab register_spec_statement_cmd]
+-- unsafe def register_spec_statement : Lean.Elab.Command.CommandElab := fun stx => do
+--   let bla := stx[1]
+--   let expr ← Command.liftTermElabM do
+--     elabTerm bla (some (mkConst ``SpecInfo))
+--   let value ← Lean.Elab.Command.liftTermElabM do
+--     Lean.Meta.evalExpr SpecInfo (mkConst ``SpecInfo) expr
+--   specAttr.add value
+
+-- details that are specific to particular kinds of spec statements, like `spec` of `dspec`
+-- unsafe def specStatementLookup : Name → SpecInfo
+--   | ``Std.WP.spec => {
+--     name := ``Std.WP.spec
+--     arity := 3
+--     mk_spec_mono := fun _args thm => thm
+--     mk_spec_bind := fun _args thm => thm
+--     uncurry_elim_tactics := #[]
+--     qimp_elim_tactics := #[]
+--     program_index := 1
+--   }
+--   | ``Std.WP.dspec => {
+--     name := ``Std.WP.dspec
+--     arity := 3
+--     mk_spec_mono := fun _args thm => thm
+--     mk_spec_bind := fun _args thm => thm
+--     uncurry_elim_tactics := #[]
+--     qimp_elim_tactics := #[]
+--     program_index := 1
+--   }
+--   | _ => panic! "not a valid spec statement"
+
+
+end Aeneas
